partial nd with lists making sense

examples/layeredeffects/ND.fst
@@ -11,69 +11,45 @@ module F = FStar.FunctionalExtensionality
 module W = FStar.WellFounded
 module T = FStar.Tactics
 
-// m is a monad
+// m is a monad. In this particular example, lists
 val m (a : Type u#a) : Type u#a
 let m a = list a
 
-val m_return (a : Type) : a -> m a
-let m_return a x = [x]
+val m_return (#a : Type) : a -> m a
+let m_return x = [x]
 
-val m_bind (a : Type) (b : Type) : m a -> (a -> m b) -> m b
-let m_bind _ _ =
-  fun l f -> concatMap f l
+val m_bind (#a #b : Type) : m a -> (a -> m b) -> m b
+let m_bind l f = concatMap f l
 
 // w is an ordered (w_ord) monad with conjunction (w_conj) and actions from prop (w_act_prop)
+// In this example, good ol' continuations into prop
 val w0 (a : Type u#a) : Type u#(max 1 a)
 let w0 a = (a -> Type0) -> Type0
-
 
 let monotonic (w:w0 'a) =
   forall p1 p2. (forall x. p1 x ==> p2 x) ==> w p1 ==> w p2
 
 val w (a : Type u#a) : Type u#(max 1 a)
-let w a = w:(w0 a){monotonic w}
+let w a = w:(w0 a)//{monotonic w}
 
+val w_ord (#a : Type) : w a -> w a -> Type0
+let w_ord wp1 wp2 = forall p. wp1 p ==> wp2 p
 
-val w_ord (a : Type) : w a -> w a -> Type0
-let w_ord a wp1 wp2 = forall p. wp1 p ==> wp2 p
+unfold
+val w_return (#a : Type) : a -> w a
+unfold
+let w_return x = fun p -> p x
 
-val w_ord_trans (a : Type) (wp1 : w a) (wp2 : w a) (wp3 : w a) : Lemma (requires w_ord a wp1 wp2 /\ w_ord a wp2 wp3) (ensures w_ord a wp1 wp3)
-let w_ord_trans = fun _ _ _ _ -> ()
-
-// GM: this is "assume"
-val w_act_prop (a : Type) : Type0 -> w a -> w a
-let w_act_prop a phi wp = fun p -> phi ==> wp p
-
-
-val w_conj (a : Type) : w a -> w a -> w a
-let w_conj a wp1 wp2 p = wp1 p /\ wp2 p
-
-val w_return (a : Type) : a -> w a
-let w_return a x = fun p -> p x
-
-val w_bind (a : Type) (b : Type) : w a -> (a -> w b) -> w b
-let w_bind a b wp1 k =
+unfold
+val w_bind (#a #b : Type) : w a -> (a -> w b) -> w b
+unfold
+let w_bind wp1 k =
   fun p -> wp1 (fun x -> k x p)
 
-val w_bind_monotonic (a : Type) (b : Type) (m1 : w a) (m2 : w a) (f1 : a -> w b) (f2 : a -> w b) : Lemma (requires w_ord a m1 m2 /\ (forall (a : a).{:pattern f2 a} w_ord b (f1 a) (f2 a))) (ensures w_ord b (w_bind a b m1 f1) (w_bind a b m2 f2))
-let w_bind_monotonic a b m1 m2 f1 f2 = ()
-
-// we can define an "equality" on w a
-val w_equiv (a : Type) : w a -> w a -> Type0
-let w_equiv a wp1 wp2 = w_ord a wp1 wp2 /\ w_ord a wp2 wp1
-
-// the monad morphism that connect the two monadic structures
 val interp (#a : Type) : m a -> w a
-
-let interp #a (l:list a) =
-  fun p -> forall x. memP x l ==> p x
-
-val interp_ret (a : Type) (x : a) : Lemma (interp (m_return a x) `w_equiv a` w_return a x)
-let interp_ret a x = ()
-
+let interp #a (l:list a) = fun p -> forall x. memP x l ==> p x
 
 val concatlemma (#a:Type) (l1 l2 :list a) (x:a) : Lemma (memP x (l1@l2) <==> memP x l1 \/ memP x l2)
-
 let rec concatlemma #a l1 l2 x =
   match l1 with
   | [] -> ()
@@ -90,109 +66,68 @@ let rec concatmaplemma #a #b l f x =
     concatlemma (f h) (concatMap f t) x;
     concatmaplemma t f x
 
-
-let dro_w a wp2 wp1 = w_ord a wp1 wp2
-
-val interp_bind (a b : Type) (v : m a) (f : a -> m b) : Lemma (interp (m_bind a b v f) `w_equiv _` w_bind a b (interp v) (fun a -> interp (f a)))
-
-// uses pattern above, slightly brittle too
-#push-options "--retry 10"
-let interp_bind a b v f = ()
-#pop-options
-
-// In DM4A we would have something like:
-
-// total
-// reifiable
-// reflectable
-// new_effect {
-//   DM4A : a:Type -> Effect
-//   with
-//        repr      = m
-//      ; return    = m_return
-//      ; bind      = m_bind
-
-//      ; wp_type   = w
-//      ; return_wp = w_return
-//      ; bind_wp   = w_bind
-
-//      ; interp    = interp
-// }
-
-// In layered effects, we instead construct the Dijkstra monad as a
-// sigma type (see the paper)
-
-let dm (a : Type) (wp : w a) : Type = v:m a{w_ord a wp (interp v)}
-
-let irepr (a : Type) (wp: w a) = unit -> dm a wp
-let ireturn (a : Type) (x : a) : irepr a (w_return a x) = fun () -> interp_ret a x ; m_return a x
-
-let ibind (a : Type) (b : Type) (wp_v : w a) (wp_f: a -> w b) (v : irepr a wp_v) (f : (x:a -> irepr b (wp_f x))) : irepr b (w_bind a b wp_v 
-wp_f) =
-  fun () ->
-  interp_bind a b (v ()) (fun x -> f x ()) ;
-  w_bind_monotonic a b wp_v (interp (v ())) wp_f (fun a -> interp (f a ()));
-  w_ord_trans b (w_bind a b wp_v wp_f) (w_bind a b (interp (v ())) (fun a -> interp (f a ()))) (interp (m_bind a b (v ()) (fun x -> f x ())));
-  m_bind a b (v ()) (fun x -> f x ())
- 
-let isubcomp (a:Type) (wp1 wp2: w a) (f : irepr a wp1) : Pure (irepr a wp2) (requires w_ord a wp2 wp1) (ensures fun _ -> True) =
-  fun () -> w_ord_trans a wp2 wp1 (interp (f ())) ; f () 
-
-let wp_if_then_else (a:Type) (wp1 wp2:w a) (p:bool) : w a=
-  w_conj a (w_act_prop a p wp1) (w_act_prop a (~p) wp2)
-
-let i_if_then_else (a : Type) (wp1 wp2 : w a) (f : irepr a wp1) (g : irepr a wp2) (p : bool) : Type =
-  irepr a (wp_if_then_else a wp1 wp2 p)
-
-let lem_if_1 (a:Type) (wp1 wp2 : w a) (p:bool) (f : irepr a wp1) (g : irepr a wp2)
-  : Lemma (p ==> w_ord a (wp_if_then_else a wp1 wp2 p) wp1)
-          [SMTPat ()]
-  = 
-  let aux post : Lemma (requires p /\ wp_if_then_else a wp1 wp2 p post)
-                       (ensures wp1 post)
-    =
-    calc (<==>) {
-      wp1 post;
-      <==> {}
-      p ==> wp1 post;
-      <==> {}
-      (p ==> wp1 post) /\ ((~p) ==> wp2 post);
-      <==> {}
-      (w_act_prop a p wp1 post) /\ (w_act_prop a (~p) wp2 post);
-      <==> { _ by (compute ()) } // GM: why???
-      w_conj a (w_act_prop a p wp1) (w_act_prop a (~p) wp2) post;
-      <==> {}
-      wp_if_then_else a wp1 wp2 p post;
-    }
-  in
-  Classical.forall_intro (Classical.move_requires aux)
+let dm (a : Type) (wp : w a) : Type = 
+  p:(a -> Type0) -> squash (wp p) -> l:(m a){forall x. memP x l ==> p x}
   
-let lem_if_2 (a:Type) (wp1 wp2 : w a) (p:bool) (f : irepr a wp1) (g : irepr a wp2)
-  : Lemma ((~p) ==> w_ord a (wp_if_then_else a wp1 wp2 p) wp2)
-          [SMTPat ()]
-  = 
-  let aux post : Lemma (requires (~p) /\ wp_if_then_else a wp1 wp2 p post)
-                       (ensures wp2 post)
-    =
-    calc (<==>) {
-      wp2 post;
-      <==> {}
-      (~p) ==> wp2 post;
-      <==> {}
-      (p ==> wp1 post) /\ ((~p) ==> wp2 post);
-      <==> {}
-      (w_act_prop a p wp1 post) /\ (w_act_prop a (~p) wp2 post);
-      <==> { _ by (compute ()) } // GM: why???
-      w_conj a (w_act_prop a p wp1) (w_act_prop a (~p) wp2) post;
-      <==> {}
-      wp_if_then_else a wp1 wp2 p post;
-    }
-  in
-  Classical.forall_intro (Classical.move_requires aux)
+let irepr (a : Type) (wp: w a) = dm a wp
 
-// requires to prove that
-// p ==> subcomp f (if_then_else p f g)
+let ireturn (a : Type) (x : a) : irepr a (w_return x) = fun _ _ -> [x]
 
+let rec pmap #a #b #pre (#post:b->Type0)
+  (f : (x:a -> Pure b (requires (pre x)) (ensures post)))
+  (l : list a)
+  : Pure (list (v:b{post v}))
+         (requires (forall x. memP x l ==> pre x))
+         (ensures (fun _ -> True))
+  = match l with
+    | [] -> []
+    | x::xs -> f x :: pmap #_ #_ #pre #post f xs
+
+let rec unref #a #p (l : list (v:a{p v})) : l:(list a){forall x. memP x l ==> p x} =
+  match l with
+  | [] -> []
+  | x :: xs -> x :: unref xs
+
+let mem_memP
+  (#a: eqtype)
+  (x: a)
+  (l: list a)
+: Lemma (ensures (mem x l <==> memP x l))
+        [SMTPat (memP x l); SMTPat (mem x l)]
+= FStar.List.Tot.Properties.mem_memP x l
+
+val append_memP: #t:Type ->  l1:list t
+              -> l2:list t
+              -> a:t
+              -> Lemma (requires True)
+                       (ensures (memP a (l1@l2) <==> (memP a l1 \/ memP a l2)))
+let rec append_memP #t l1 l2 a = match l1 with
+  | [] -> ()
+  | hd::tl -> append_memP tl l2 a
+
+let rec flatten_mem_lem #a (l : list (list a)) (x:a)
+  : Lemma (memP x (flatten l) <==> (exists l0. memP l0 l /\ memP x l0))
+          [SMTPat (memP x (flatten l))]
+  = match l with
+    | [] -> ()
+    | l1::ls -> (append_memP l1 (flatten ls) x; flatten_mem_lem ls x)
+
+let ibind (a : Type) (b : Type) (wp_v : w a) (wp_f: a -> w b) (v : irepr a wp_v) (f : (x:a -> irepr b (wp_f x))) : irepr b (w_bind wp_v wp_f) =
+  fun p _ -> let l1 = v (fun x -> wp_f x p) () in
+          let l2 = pmap #_ #(list b) #(fun x -> wp_f x p) #(fun l -> forall x. memP x l ==> p x) (fun x -> f x p ()) l1 in
+          let l2 = unref l2 in
+          let l2f = List.Tot.flatten l2 in
+          l2f
+ 
+let isubcomp (a:Type) (wp1 wp2: w a) (f : irepr a wp1) : Pure (irepr a wp2) (requires w_ord wp2 wp1) (ensures fun _ -> True) = f
+
+let wp_if_then_else (#a:Type) (wp1 wp2:w a) (b:bool) : w a=
+  fun p -> (b ==> wp1 p) /\ ((~b) ==> wp2 p)
+
+let i_if_then_else (a : Type) (wp1 wp2 : w a) (f : irepr a wp1) (g : irepr a wp2) (b : bool) : Type =
+  irepr a (wp_if_then_else wp1 wp2 b)
+
+total
 reifiable
 reflectable
 layered_effect {
@@ -204,53 +139,32 @@ layered_effect {
        if_then_else = i_if_then_else
 }
 
-assume Mono : forall (a:Type) (wp:pure_wp a). monotonic wp
-
-assume Pure_wp_corr : forall (a:Type) (wp:pure_wp a) (f:(unit -> PURE a wp))
-                        (p:pure_post a). wp p ==> p (f ())
-
-let lemgg (a:Type) (wp:pure_wp a) p q (_ : squash p) (_ : monotonic wp) :
-    Lemma (requires (wp (fun _ -> p)))
-          (ensures (wp (fun x -> q x ==> p))) = ()
-
-let lemhh (a:Type) (wp:pure_wp a) p (_ : squash p) :
-    Lemma (requires (wp (fun _ -> True)))
-          (ensures (wp (fun _ -> p))) = ()
-
-(*
- * AR: With the stricter check on the types of layered effects combinators,
- *     lift_pure_nd no longer typechecks, since irepr expects a (w a),
- *     which is not definitionally (pure_wp a)
- *
- *     Working aroung with this coercion
- *)
-
-#push-options "--admit_smt_queries true"
-let coerce_pure_wp (#a:Type) (wp:pure_wp a) : w a = wp
-#pop-options
-
 let lift_pure_nd (a:Type) (wp:pure_wp a) (f:(eqtype_as_type unit -> PURE a wp)) :
-  Pure (irepr a (coerce_pure_wp wp)) (requires (wp (fun _ -> True)))
+  Pure (irepr a wp) (requires True)
                     (ensures (fun _ -> True))
-  = fun () -> admit (); [f ()] // GM : not sure why this fails
+  = fun p _ -> let r = Common.elim_pure f p in [r]
 
 sub_effect PURE ~> ND = lift_pure_nd
 
+val test_f : unit -> ND int (fun p -> p 5 /\ p 3)
+let test_f () =
+  ND?.reflect (fun _ _ -> [3; 5])
 
-assume val test_f : unit -> ND int (fun p -> p 5 /\ p 3)
+//let l () : (l:(list int){forall p. p 5 /\ p 3 ==> interp l p}) = reify (test_f ())
+// ^ This one doesn't work... datatype subtyping to blame?
 
-let l : unit -> (l:list int{forall p. p 5 /\ p 3 ==> interp l p}) = reify (test_f ())
+let l () : (l:(list int)) = reify (test_f ()) (fun _ -> True) ()
 
 effect Nd (a:Type) (pre:pure_pre) (post:pure_post' a pre) =
         ND a (fun (p:pure_post a) -> pre /\ (forall (pure_result:a). post pure_result ==> p pure_result))
 
 val choose : #a:Type0 -> x:a -> y:a -> ND a (fun p -> p x /\ p y)
 let choose #a x y =
-    ND?.reflect (fun () -> [x;y])
+    ND?.reflect (fun _ _ -> [x;y])
 
 val fail : #a:Type0 -> unit -> ND a (fun p -> True)
 let fail #a () =
-    ND?.reflect (fun () -> [])
+    ND?.reflect (fun _ _ -> [])
 
 let flip () : ND bool (fun p -> p true /\ p false) =
     choose true false
@@ -300,4 +214,9 @@ let (pyths_norm : unit -> (Prims.int * Prims.int * Prims.int) Prims.list) =
     ((Prims.parse_int "6"), (Prims.parse_int "8"), (Prims.parse_int "10"));
     ((Prims.parse_int "8"), (Prims.parse_int "6"), (Prims.parse_int "10"))]
 *)
-let pyths_norm () = normalize_term (reify (pyths ()) ())
+let pyths_norm () = normalize_term (reify (pyths ()))
+
+(* ^ Try it in emacs: C-c C-s C-e pyths_norm ():
+Reducing ‘pyths_norm ()’…
+pyths_norm () ↓βδιζr [3, 4, 5; 4, 3, 5; 6, 8, 10; 8, 6, 10] <: list ((int * int) * int)
+*)
