examples/layeredeffects/Common.fst
@@ -1,0 +1,10 @@
+module Common
+
+(* Common lemmas and constructions for layered effects examples. *)
+
+let elim_pure #a #wp ($f : unit -> PURE a wp) p
+ : Pure a (requires (wp p)) (ensures (fun r -> p r))
+ //: PURE a (fun p' -> wp p /\ (forall r. p r ==> p' r))
+ // ^ basically this, requires monotonicity
+ = FStar.Monotonic.Pure.wp_monotonic_pure ();
+   f ()
